\documentclass{article}
\usepackage{ifthen}
\usepackage{epsfig}
\usepackage[utf8]{inputenc}
\usepackage{xcolor}
% Packages requested by user
\usepackage{amsmath}
\usepackage{amssymb}

\usepackage{newunicodechar}
  \newunicodechar{⁻}{${}^{-}$}% Superscript minus
  \newunicodechar{²}{${}^{2}$}% Superscript two
  \newunicodechar{³}{${}^{3}$}% Superscript three

\pagestyle{empty}
\begin{document}
$ dN(r)/d\ln r $
\pagebreak

$ dM(r,s)/d\ln r $
\pagebreak

$V$
\pagebreak

$R_{\rm geo}$
\pagebreak

$D_{\rm geo}$
\pagebreak

$N$
\pagebreak

$R_{\rm me}$
\pagebreak

$\rm
   s^{-1}$
\pagebreak

$N_{\rm back}$
\pagebreak

$\dot{N} = r N_{\rm back} - r N$
\pagebreak

$r$
\pagebreak

$t_i$
\pagebreak

$r_i$
\pagebreak

$a_i$
\pagebreak

$i = 1,\ldots,n$
\pagebreak

$t_{i+1}$
\pagebreak

$r_i a_i$
\pagebreak

$t_1$
\pagebreak

$r_1 a_1$
\pagebreak

$t_n$
\pagebreak

$r_n a_n$
\pagebreak

\[ n(v) = \frac{1}{\rm mean-vol} \exp(- v / {\rm mean-vol}) \]
\pagebreak

$N + 1$
\pagebreak

$D_1,\ldots,D_{N+1}$
\pagebreak

$D_i < D_{i+1}$
\pagebreak

$C_1,\ldots,C_N$
\pagebreak

$C_i$
\pagebreak

$[D_i, D_{i+1}]$
\pagebreak

\[ n(\log D) {\rm d}\log D
      = \frac{N_{\rm total}}{\sqrt{2\pi} \log \sigma_{\rm g}}
      \exp\left(\frac{(\log D - \log D_{\rm gn})^2}{2 \log ^2
      \sigma_{\rm g}}\right)
      {\rm d}\log D \]
\pagebreak

$N_{\rm total}$
\pagebreak

$D_{\rm gn}$
\pagebreak

$\log_{10}$
\pagebreak

$\sigma_{\rm g}$
\pagebreak

\[ n(v) {\rm d}v = \frac{N_{\rm total}}{v_{\rm \mu}}
      \exp\left(- \frac{v}{v_{\rm \mu}}\right)
      {\rm d}v \]
\pagebreak

$D_{\rm \mu}$
\pagebreak

$v_{\rm \mu}
           = \frac{\pi}{6} D^3_{\rm \mu}$
\pagebreak

$D_0$
\pagebreak

$R_0$
\pagebreak

$D_0 = 2 R_0$
\pagebreak

$f(D)$
\pagebreak

\[
     f(D) = D^6 + c_4 D^4 + c_3 D^3 + c_0,
 \]
\pagebreak

$c_4 < 0$
\pagebreak

$c_3 < 0$
\pagebreak

$c_0 > 0$
\pagebreak

$D > D_{\rm dry}$
\pagebreak

\[
     f'(D) = 6 D^5 + 4 c_4 D^3 + 3 c_3 D^2
           = (3 D^2 + 4 c_4) D^3 + (D^3 + c_3) 3 D^2.
 \]
\pagebreak

$D > (-4 c_4 / 3)^{1/2}$
\pagebreak

$D > (-c_3)^{1/3}$
\pagebreak

\[
     D_0 = max((-4 c_4 / 3)^{1/2}, (-c_3)^{1/3})
 \]
\pagebreak

$f'(D) > 0$
\pagebreak

$D > D_0$
\pagebreak

\[
     f''(D) = 30 D^4 + 12 c_4 D^2 + 6 c_3 D
            = (5 D^2 + 4 c_4) 3 D^2 + (5 D^3 + 2 c_3) 3 D,
 \]
\pagebreak

$f''(D) > 0$
\pagebreak

$D
 > (-4 c_4 / 5)^{1/2}$
\pagebreak

$D > (-2 c_3 / 5)^{1/3}$
\pagebreak

$n(D)$
\pagebreak

\[ n(D) = w(D) c(D) \]
\pagebreak

$w(D)$
\pagebreak

$c(D)$
\pagebreak

$D$
\pagebreak

$w(D) = 1$
\pagebreak

$w(D) = D^\alpha$
\pagebreak

$w(D) =
     D^{-3}$
\pagebreak

$\alpha$
\pagebreak

$w(D) =
     (D/D_0)^\alpha$
\pagebreak

$w(D) =
     (D/D_0)^{-3}$
\pagebreak

$n_{\rm bin}$
\pagebreak

$c_i$
\pagebreak

$i =
 1,\ldots,n_{\rm bin}$
\pagebreak

$e_i$
\pagebreak

$i =
 1,\ldots,(n_{\rm bin} + 1)$
\pagebreak

$e_{i+1}/e_i$
\pagebreak

$c_i/e_i = \sqrt{e_{i+1}/e_i}$
\pagebreak

$\ln(e_i)$
\pagebreak

$\ln(c_i)$
\pagebreak

$e_1$
\pagebreak

$e_{n_{\rm bin} + 1}$
\pagebreak

$k_{\rm D}$
\pagebreak

$ \delta = k_{\rm D}(D/D_0)^a $
\pagebreak

$ \delta $
\pagebreak

$a$
\pagebreak

$R$
\pagebreak

$N_0$
\pagebreak

$v_\mu = \frac{4\pi}{3} R^3$
\pagebreak

$\tau = N_0 v_\mu \beta_1 t$
\pagebreak

$T = 1 -
 e^{-\tau}$
\pagebreak

$\beta_1$
\pagebreak

\[
     n(D,t) \ {\rm d}\ln D
     = \frac{\pi}{2} D^3
       \frac{N_0}{v} \frac{1 - T}{\sqrt{T}}
       \exp\left(-(1 + T) \frac{v}{v_\mu}\right)
       I_1\left(2 \frac{v}{v_\mu} \sqrt{T}\right) {\rm d}\ln D
 \]
\pagebreak

$I_1(x)$
\pagebreak

$v = \frac{\pi}{6}
 D^3$
\pagebreak

$x$
\pagebreak

$I_1(x) \approx \frac{x}{2}$
\pagebreak

\[
     n(D,t) \ {\rm d}\ln D
     = \frac{\pi}{2} D^3 \frac{N_0}{v_\mu}
     \exp\left(-\frac{v}{v_\mu}\right) {\rm d}\ln D
 \]
\pagebreak

$ I_1(x) $
\pagebreak

$\tau = N_0 \beta_0 t$
\pagebreak

$\beta_0$
\pagebreak

$\lambda = 1$
\pagebreak

\[
     n(D,t) \ {\rm d}\ln D
     = \frac{\pi}{2} D^3 \frac{N_0}{v_\mu} \frac{4}{(\tau + 2)^2}
     \exp\left(-\frac{v}{v_\mu} \frac{2}{\tau + 2}
     \exp(-\lambda \tau) - \lambda \tau\right) {\rm d}\ln D
 \]
\pagebreak

$n(D,t)$
\pagebreak

$t$
\pagebreak

\[
     \frac{d n(D,t)}{dt} = k_{\rm emit} n_{\rm emit}(D)
         + (k_{\rm dilute} + k_{\rm loss}(D)) (n_{\rm back}(D) - n(D,t))
 \]
\pagebreak

$ n(D,0) = n_0(D) $
\pagebreak

$n_{\rm emit}(D)$
\pagebreak

$n_{\rm back}(D)$
\pagebreak

$k_{\rm
 emit}$
\pagebreak

$k_{\rm dilute}$
\pagebreak

$k_{\rm loss}(D)$
\pagebreak

$t = 0$
\pagebreak

\[
     n(D,t) = n_{\infty}(D)
              + (n_0(D) - n_{\infty}(D)) \exp(
                                -(k_{\rm dilute} + k_{\rm loss}(D)) t)
 \]
\pagebreak

\[
     n_{\infty}(D) = n(D,\infty)
                   = n_{\rm back}(D)
                     + \frac{k_{\rm emit}}{k_{\rm dilute}
                       + k_{\rm loss}(D)} n_{\rm emit}(D)
 \]
\pagebreak

$ T $
\pagebreak

$ p $
\pagebreak

$ D_i $
\pagebreak

$ H $
\pagebreak

$ (D_1,\ldots,D_n,H)
 $
\pagebreak

$(I - \gamma J) x = b$
\pagebreak

$J$
\pagebreak

$\gamma$
\pagebreak

$b$
\pagebreak

$A$
\pagebreak

$Q$
\pagebreak

$z$
\pagebreak

$d_{\rm f}$
\pagebreak

$R_{\rm 0}$
\pagebreak

$f$
\pagebreak

$d_{\rm s}$
\pagebreak

$S_{\rm acc}$
\pagebreak

$h_{\rm KR}$
\pagebreak

$R_{\rm me,c}$
\pagebreak

$R_{\rm eff}$
\pagebreak

$C(R_eff)$
\pagebreak

$g_i$
\pagebreak

$r_i g_i$
\pagebreak

$r_1 g_1$
\pagebreak

$r_n
 g_n$
\pagebreak

$\rm H_2SO_4$
\pagebreak

$\rm
 SO_2$
\pagebreak

$4\times
 10^{-9}\rm\ mol\ m^{-2}\ s^{-1}$
\pagebreak

$2.8\times
 10^{-9}\rm\ mol\ m^{-2}\ s^{-1}$
\pagebreak

$5\times
 10^{-9}\rm\ mol\ m^{-2}\ s^{-1}$
\pagebreak

$i$
\pagebreak

$j$
\pagebreak

$k$
\pagebreak

$\mathbb{Z} \to \mathbb{Z} \times \mathbb{Z}$
\pagebreak

$\{1,
 \ldots, N_{\rm d}\}$
\pagebreak

$(j_1,j_2)$
\pagebreak

$\{1, \ldots, N_{\rm r,1} \times \{1, \ldots, N_{\rm
 r,2}\}$
\pagebreak

$(j_1, j_2)$
\pagebreak

$ J = K H^2 $
\pagebreak

$H$
\pagebreak

$ \rm H_2SO_4 $
\pagebreak

$K$
\pagebreak

\[ | A_1 - A_2 |_2 < \verb+abs_tol+ \]
\pagebreak

\[ \frac{| A_1 - A_2 |_2}{| A_1 |_2 + | A_2 |_2}
           < \verb+rel_tol+ \]
\pagebreak

$np \le 10$
\pagebreak

$n(1-p) \le 10$
\pagebreak

$[0,1)$
\pagebreak

$[1,n]$
\pagebreak

$e(t)$
\pagebreak

$h(t)$
\pagebreak

$r(t)$
\pagebreak

$c(t)$
\pagebreak

\[
     c(t) = c(0) + \frac{r t}{h} e.
 \]
\pagebreak

$\lambda(t)$
\pagebreak

\[
     \lambda_{\rm eff}(t) = \lambda(t) + \frac{\dot{h}(t)}{h(t)}
 \]
\pagebreak

\[
     \dot{c}(t) = - \lambda_{\rm eff}(t) c(t).
 \]
\pagebreak

\[
     \frac{c(t)}{c(0)} = \frac{h(0)}{h(t)}
                         \exp\left( - \int_0^t \lambda(t)\,dt\right).
 \]
\pagebreak

$p = c(t)/c(0)$
\pagebreak

\[
     c(t) = p(t) c(0) + (1 - p(t)) b.
 \]
\pagebreak

$\lambda$
\pagebreak

\[
     p(t) = \min\left(1, \frac{h(0)}{h(t)}\right) \exp(-\lambda t).
 \]
\pagebreak

$m_1 = x_1$
\pagebreak

$v_1 = 0$
\pagebreak

$n = 1$
\pagebreak

$n \ge 2$
\pagebreak

\[
     m_n = m_{n-1} + \frac{x_n - m_{n-1}}{n}
 \]
\pagebreak

\[
     v_n = \frac{n - 2}{n - 1} v_{n-1}
           + \frac{(x_n - m_{n-1})^2}{n}.
 \]
\pagebreak

$m_n$
\pagebreak

$v_n$
\pagebreak

$\{x_1,\ldots,x_n\}$
\pagebreak

$n$
\pagebreak

\[
     t_n = \sum_{i=1}^n x_i
 \]
\pagebreak

\[
     s_n = \sum_{i=1}^n (x_i - m_n)^2.
 \]
\pagebreak

$m_n = \frac{t_n}{n}$
\pagebreak

$p_n = \frac{1}{n} \left( s_n - n m_n^2
 \right)$
\pagebreak

$v_n = \frac{1}{n -
 1} \left( s_n - n m_n^2 \right)$
\pagebreak

\[
     s_n = \sum_{i=1}^n x_i^2 - n m_n^2
 \]
\pagebreak

\[
     s_n = s_{n-1} + \frac{n - 1}{n} (x_n - m_{n-1})^2.
 \]
\pagebreak

\[
     p_n = \frac{n-1}{n} p_{n-1} + \frac{(x_n - m_n)(x_n - m_{n-1})}{n}
         = \frac{n-1}{n} p_{n-1} + \frac{n-1}{n^2} (x_n - m_{n-1})^2.
 \]
\pagebreak

$s_n$
\pagebreak

$n \kappa \epsilon$
\pagebreak

$\epsilon$
\pagebreak

$\kappa$
\pagebreak

\[
     \kappa = \frac{\|x\|_2}{\sqrt{s_n}}
            = \sqrt{1 + \frac{m_n^2}{p_n}}
            \approx \frac{m_n}{p_n}.
 \]
\pagebreak

$m_{n-1}$
\pagebreak

$v_{n-1}$
\pagebreak

$x_n$
\pagebreak

$\mu$
\pagebreak

$\sigma$
\pagebreak

$[\mu - r\sigma/\sqrt{n}, \mu +
 r\sigma/\sqrt{n}]$
\pagebreak

$f(\nu) =
 t_{0.95,\nu}$
\pagebreak

$\nu = n - 1$
\pagebreak

$g(\nu) = f(\nu)
 - L$
\pagebreak

$L = \Phi^{-1}(0.975)$
\pagebreak

$\Phi$
\pagebreak

$g'(\nu) < -1$
\pagebreak

$g'(\nu) \to -1$
\pagebreak

$\nu \to
 \infty$
\pagebreak

$g(\nu)$
\pagebreak

$A/\nu$
\pagebreak

$g(\nu^*) = A^*/\nu$
\pagebreak

$g(\nu) < A^*/\nu$
\pagebreak

$\nu > \nu^*$
\pagebreak

$f(\nu) \le (f(\nu^*) - L) (\nu^* / \nu) + L$
\pagebreak

$\nu \ge
 \nu^*$
\pagebreak

$(\nu^*, f(\nu^*))$
\pagebreak

$l$
\pagebreak

$ \ell_1 $
\pagebreak

$ - p \ln p$
\pagebreak

$p$
\pagebreak

\end{document}
